Sketch in a spec based on our Dafny spec for AES

src/crypto/aes/AES_s.fst
@@ -1,6 +1,8 @@
 module AES_s
 
 open Types_s
+open FStar.Seq
+open FStar.Mul
 
 assume val mix_columns (q:quad32) : quad32
 assume val inv_mix_columns (q:quad32) : quad32
@@ -10,3 +12,80 @@ assume val shift_rows (q:quad32) : quad32
 assume val inv_shift_rows (q:quad32) : quad32
 assume val rot_word (w:nat32) : nat32
 assume val sub_word (w:nat32) : nat32
+
+type algorithm = | AES_128 | AES_192 | AES_256
+
+let aes_rcon (i:int) =
+    if i = 0 then 0x01 else if i = 1 then 0x02 else if i = 2 then 0x04 else if i = 3 then 0x08 else if i = 4 then 0x10 else if i = 5 then 0x20 else if i = 6 then 0x40 else if i = 7 then 0x80 else if i = 8 then 0x1b else 0x36
+
+// AES fixes Rijndael's block size at 4 32-bit words
+let nb = 4
+
+// Number of key words
+unfold let nk(alg:algorithm) =
+  match alg with
+  | AES_128 -> 4
+  | AES_192 -> 6
+  | AES_256 -> 8
+
+// Number of rounds
+unfold let nr(alg:algorithm) =
+  match alg with
+  | AES_128 -> 10
+  | AES_192 -> 12
+  | AES_256 -> 14
+
+let round (state round_key:quad32) =
+  let s = sub_bytes state in
+  let s = shift_rows s in
+  let s = mix_columns s in
+  let s = quad32_xor s round_key in
+  s
+
+let rec rounds (state:quad32) (round_keys:seq quad32)
+               (start:nat) (last:nat{start <= last /\ last < length round_keys}) : Tot quad32 (decreases %[last - start]) =
+  if start = last then 
+    state
+  else
+    rounds (round state (index round_keys start)) round_keys (start + 1) last
+
+let cipher (alg:algorithm) (input:quad32) (round_keys:seq quad32{length round_keys == (nr alg) + 1}) = 
+  let state = quad32_xor input (index round_keys 0) in
+  let state = rounds state round_keys 1 (nr alg) in
+  let state = sub_bytes state in
+  let state = shift_rows state in
+  let state = quad32_xor state (index round_keys (nr alg)) in
+  state
+
+let nat32_xor (x y:nat32) : nat32 = FStar.UInt.logxor #32 x y
+
+let rec expand_key (alg:algorithm) (key:seq nat32 { length key == nk alg}) (size:nat{size <= (nb * ((nr alg) + 1))})
+  : (ek:seq nat32 {length ek == size}) =
+  if size = 0 then createEmpty
+  else
+    let w = expand_key alg key (size - 1) in
+    let i = size - 1 in
+    if 0 <= i && i < nk alg then
+      append w (create 1 (index key i))
+    else
+      let temp = 
+        if i % (nk alg) = 0 then
+	  nat32_xor (sub_word (rot_word (index w (i-1)))) (aes_rcon ((i / (nk alg)) - 1))
+	else if nk alg > 6 && i % (nk alg) = 4 then
+	  sub_word (index w (i-1))
+	else
+	  index w (i-1)
+      in 
+      append w (create 1 (nat32_xor (index w (i - (nk alg))) temp))
+	 
+let rec key_schedule_to_round_keys (rounds:nat) (w:seq nat32 {length w >= 4 * rounds}) 
+  : (round_keys:seq quad32 {length round_keys == rounds}) =
+  if rounds = 0 then createEmpty
+  else 
+    let round_keys = key_schedule_to_round_keys (rounds - 1) w in
+    let rk = Quad32 (index w (4 * rounds - 4)) (index w (4 * rounds - 3)) (index w (4 * rounds - 2)) (index w (4 * rounds - 1)) in
+    append round_keys (create 1 rk)
+
+let aes_encrypt (alg:algorithm) (key:seq nat32 {length key == nk alg}) (input:quad32) =
+  cipher alg input (key_schedule_to_round_keys (nr alg + 1) (expand_key alg key (nb * (nr alg + 1))))
+
